model/basic/interference_edf.v
@@ -55,6 +55,44 @@ Module InterferenceEDF.
       }
     Qed.
 
+    (* Under EDF scheduling, a job only causes interference if its deadline
+       is not larger than the deadline of the analyzed job. *)
+    Lemma interference_with_parallelism_under_edf_implies_shorter_deadlines :
+      forall (j j': JobIn arr_seq) t1 t2,
+        job_interference_with_parallelism job_cost sched j' j t1 t2 != 0 ->
+        job_arrival j + job_deadline j <= job_arrival j' + job_deadline j'.
+    Proof.
+      rename H_scheduler_uses_EDF into PRIO.
+      intros j j' t1 t2 INTERF.
+      unfold job_interference_with_parallelism in INTERF.
+      destruct ([exists t': 'I_t2,
+                   [exists cpu: processor num_cpus,
+                      (t' >= t1) && backlogged job_cost sched j' t' &&
+                                              scheduled sched j t']]) eqn:EX.
+      {
+        move: EX => /existsP [t' /existsP [cpu /andP [/andP [LE BACK] SCHED]]].
+        by eapply PRIO in SCHED; last by apply BACK.
+      }
+      {
+        apply negbT in EX; rewrite negb_exists in EX; move: EX => /forallP ALL.
+        rewrite big_nat_cond (eq_bigr (fun x => 0)) in INTERF;
+          first by rewrite -big_nat_cond big_const_nat iter_addn mul0n  addn0 eq_refl in INTERF.
+        move => i /andP [/andP [GEi LTi] _].
+        specialize (ALL (Ordinal LTi)).
+        rewrite negb_exists in ALL.
+        move: ALL => /forallP ALL.
+        rewrite (eq_bigr (fun x => 0));
+          first by rewrite big_const_ord iter_addn mul0n addn0.
+        intros cpu _; specialize (ALL cpu); simpl in ALL.
+        destruct (backlogged job_cost sched j' i); last by rewrite andFb.
+        rewrite GEi 2!andTb in ALL; rewrite andTb.
+        rewrite negb_exists in ALL; move: ALL => /forallP NOTSCHED.
+        specialize (NOTSCHED cpu); rewrite negb_and in NOTSCHED.
+        move: NOTSCHED => /orP [BUG | NOTSCHED]; first by done.
+        by apply/eqP; rewrite eqb0.  
+      }
+    Qed.
+    
   End Lemmas.
 
 End InterferenceEDF.
